Finished mwov_prefix and polished some other proofs.

Isabelle/Grammar_defs.thy
@@ -78,7 +78,7 @@ function minimal_word_of_variables ::
   "('t :: linorder, 'v :: linorder) grammar \<Rightarrow> 'v list \<Rightarrow> 't list" where
   "minimal_word_of_variables gr [] = []"
 | "minimal_word_of_variables gr (vh#vt) = (
-     if gram_valid (* TODO! use gram_normed here! *) gr \<and> set (vh#vt) \<subseteq> keys gr then
+     if gram_valid (* TODO! use gram_normed here! *) gr \<and> vh \<in> keys gr then
        let norms = norms_of_grammar gr in
        let (t, vars) = snd (lookup norms vh) in
        t # minimal_word_of_variables gr vars @ minimal_word_of_variables gr vt
